Tamari ordering of binary trees

theories/Combi/bintree.v
@@ -22,13 +22,27 @@ We define the following notions
 - [BinNode left right] == the binary tree with subtrees [left] [right]
 - [size_tree t] == the number of node of the tree [t]
 - [enum_bintreesz n] == the list of a trees of size [n]
+- [catalan n] == the number of binary trees of size [n]
+- [rotations t] == the list of right rotations of the tree [t]
+- [rightcomb n] == the right comb binary tree of size [n] as a [bintree]
+- [leftcomb n] == the left comb binary tree of size [n] as a [bintree]
+- [flip t] == the left/right mirror of [t]
+- [sumsizeleft t] == the sum over all node of [t] of the size of the left
+        subtree.
+
+Binary trees of size n:
+
 - [bintreesz n] == the sigma type for trees of size [n]. This is canonically
         a [finType]
-- [catalan n] == the number of binary trees of size [n]
+- [Tamari t1 t2] == [t1] is smaller than [t2] in the tamari order.
+- [rightcombsz n] == the right comb binary tree of size [n] as a [bintreesz n]
+- [leftcombsz n] == the left comb binary tree of size [n] as a [bintreesz n]
+- [flipsz t] == the left/right mirror of [t] as a [bintreesz n]
 
  *)
 Require Import mathcomp.ssreflect.ssreflect.
 From mathcomp Require Import ssrbool ssrfun bigop ssrnat eqtype fintype choice seq.
+From mathcomp Require Import fingraph path finset.
 
 Require Import tools combclass.
 
@@ -92,7 +106,7 @@ Section Size.
 Variable (n : nat).
 
 Structure bintreesz : predArgType :=
-  BintreeSZ {tval :> bintree; _ : size_tree tval == n}.
+  BinTreeSZ {tval :> bintree; _ : size_tree tval == n}.
 Canonical bintreesz_subType := Eval hnf in [subType for tval].
 Definition bintreesz_eqMixin := [eqMixin of bintreesz by <:].
 Canonical bintreesz_eqType := Eval hnf in EqType bintreesz bintreesz_eqMixin.
@@ -102,6 +116,9 @@ Canonical bintreesz_choiceType :=
 Definition bintreesz_countMixin := [countMixin of bintreesz by <:].
 Canonical bintreesz_countType :=
   Eval hnf in CountType bintreesz bintreesz_countMixin.
+
+Lemma bintreeszP (t : bintreesz) : size_tree t = n.
+Proof. by case: t => t /= /eqP. Qed.
 
 End Size.
 
@@ -287,3 +304,299 @@ rewrite /shape -map_comp -sumn_mapE; apply eq_bigr => i _.
 rewrite size_allpairs.
 by rewrite !cardT -!(size_map val) !enumT unlock !subType_seqP /=.
 Qed.
+
+Fixpoint rightcomb n :=
+  if n is n'.+1 then
+    BinNode BinLeaf (rightcomb n')
+  else BinLeaf.
+Fixpoint leftcomb n :=
+  if n is n'.+1 then
+    BinNode (leftcomb n') BinLeaf
+  else BinLeaf.
+Fixpoint flip t :=
+  if t is BinNode l r then
+    BinNode (flip r) (flip l)
+  else BinLeaf.
+
+Lemma size_rightcomb n : size_tree (rightcomb n) = n.
+Proof. elim: n => //= n ->; by rewrite addn0 add1n. Qed.
+Lemma size_leftcomb n : size_tree (leftcomb n) = n.
+Proof. elim: n => //= n ->; by rewrite addn0 add1n. Qed.
+Lemma size_flip t : size_tree (flip t) = size_tree t.
+Proof.
+elim: t => //= l -> r -> /=.
+by rewrite -!addnA [X in 1 + X]addnC.
+Qed.
+Lemma flipK : involutive flip.
+Proof. by elim => //= l -> r ->. Qed.
+Lemma flip_rightcomb n : flip (rightcomb n) = leftcomb n.
+Proof. by elim: n => //= n ->. Qed.
+Lemma flip_leftcomb n : flip (leftcomb n) = rightcomb n.
+Proof. by elim: n => //= n ->. Qed.
+
+Fixpoint rotations t :=
+  if t is BinNode l r then
+    let rec := [seq BinNode lrot r | lrot <- rotations l] ++
+               [seq BinNode l rrot | rrot <- rotations r]
+    in if l is BinNode ll lr then
+         BinNode ll (BinNode lr r) :: rec
+       else rec
+  else [::].
+
+Lemma rotation_left_sub l1 l2 r :
+  l1 \in rotations l2 -> BinNode l1 r \in rotations (BinNode l2 r).
+Proof.
+case H2 : l2 => [/= |ll2 lr2]; first by rewrite in_nil.
+rewrite -H2 /= {2}H2 => Hin.
+rewrite inE; apply/orP; right.
+rewrite mem_cat; apply/orP; left.
+by apply/mapP; exists l1.
+Qed.
+
+Lemma rotation_right_sub l r1 r2 :
+  r1 \in rotations r2 -> BinNode l r1 \in rotations (BinNode l r2).
+Proof.
+case Hl : l => [/= |ll lr] H; first by apply/mapP; exists r1.
+rewrite -Hl /= {2}Hl.
+rewrite inE; apply/orP; right.
+rewrite mem_cat; apply/orP; right.
+by apply/mapP; exists r1.
+Qed.
+
+Lemma rotationP t1 t2 :
+  reflect (exists a b c,
+              [\/ [/\ t1 = BinNode (BinNode a b) c & t2 = BinNode a (BinNode b c)],
+                  [/\ t1 = BinNode a c, t2 = BinNode b c & b \in rotations a] |
+                  [/\ t1 = BinNode a b, t2 = BinNode a c & c \in rotations b]])
+          (t2 \in rotations t1).
+Proof.
+apply (iffP idP) => [|].
+- case Ht1 : t1 => [//|[|a b] c].
+    rewrite /= => /mapP /= [rc Hrc ->].
+    by exists BinLeaf, c, rc; apply Or33.
+  rewrite [X in X -> _]/= inE => /orP [/eqP -> {t2}|].
+    by exists a, b, c; apply Or31.
+  rewrite mem_cat => /orP [/mapP [lrot] | /mapP [rrot Hrrot ->]].
+  + rewrite -[lrot \in _]/(lrot \in rotations (BinNode a b)) => Hlrot ->.
+    by exists (BinNode a b), lrot, c; apply Or32.
+  + by exists (BinNode a b), c, rrot; apply Or33.
+- move=> [a] [b] [c] [] [-> ->].
+  + by rewrite inE eq_refl.
+  + exact: rotation_left_sub.
+  + exact: rotation_right_sub.
+Qed.
+
+Lemma size_rotations t t' :
+  t' \in rotations t -> size_tree t' = size_tree t.
+Proof.
+elim: t t' => [//= | l IHl r IHr] t' /=.
+case H: l => [| ll lr] //; first by move/mapP => [/= lrot /IHr <- ->].
+rewrite inE => /orP [/eqP ->|]; first by rewrite /= !(add1n, addSn, addnS) addnA.
+by rewrite -H mem_cat => /orP [/mapP /= [lrot/IHl]|/mapP /= [rrot/IHr]] <- ->.
+Qed.
+
+Lemma rightcomb_rotations t :
+  (rotations t == [::]) = (t == rightcomb (size_tree t)).
+Proof.
+apply/eqP/eqP => [|->].
+- elim: t => [//=| l _ r IHr].
+  case: l => [| ll lr] //= Hrot.
+  have {Hrot} /IHr -> : rotations r = [::] by move: Hrot; case: (rotations r).
+  by rewrite size_rightcomb.
+- by elim: (size_tree t) => {t} //= n ->.
+Qed.
+
+Lemma rotation_flip_impl t1 t2:
+  (t1 \in rotations t2) -> (flip t2 \in rotations (flip t1)).
+Proof.
+elim: t2 t1 => [//|l IHl r IHr] t2.
+move/rotationP => [a] [b] [c] [] [H1 H2]; rewrite H1 H2.
+- by rewrite /= inE eq_refl.
+- move=> H; apply/rotationP.
+  move: H1 => [Hl Hr]; subst a; subst c => /=.
+  exists (flip r), (flip b), (flip l); apply Or33; split => //=.
+  exact: IHl.
+- move=> H; apply/rotationP.
+  move: H1 => [Hl Hr]; subst a; subst b => /=.
+  exists (flip c), (flip r), (flip l); apply Or32; split => //=.
+  exact: IHr.
+Qed.
+
+Lemma rotation_flip t1 t2:
+  (t1 \in rotations t2) = (flip t2 \in rotations (flip t1)).
+Proof.
+apply/idP/idP; first exact: rotation_flip_impl.
+by move=> /rotation_flip_impl; rewrite !flipK.
+Qed.
+
+Fixpoint sumsizeleft t :=
+  if t is BinNode l r then
+    size_tree l + sumsizeleft l + sumsizeleft r
+  else 0.
+
+Lemma sumsizeleft_gt t t' :
+  t' \in rotations t -> sumsizeleft t > sumsizeleft t'.
+Proof.
+elim: t t' => [//| l IHl r IHr] t'.
+case Hl : l IHl => [| ll lr] // IHl.
+  rewrite /= !add0n => /mapP [/= rot /IHr Hleq -> {t'}].
+  by rewrite /= !add0n.
+rewrite -Hl /= {1}Hl /= inE => /orP [/eqP -> /=|].
+  rewrite Hl /= add1n !addSn ltnS -!addnA leq_add2l.
+  rewrite !addnA !leq_add2r addnC leq_add2r.
+  exact: leq_addr.
+rewrite -Hl in IHl.
+rewrite mem_cat => /orP [/mapP /= [lrot Hlrot] | /mapP /= [rrot Hrrot]] -> /=.
+- rewrite (size_rotations Hlrot) ltn_add2r ltn_add2l.
+  exact: IHl.
+- rewrite !ltn_add2l.
+  exact: IHr.
+Qed.
+
+Lemma rotations_neq t t' : t' \in rotations t -> t != t'.
+Proof.
+move/sumsizeleft_gt; apply contraL => /eqP ->.
+by rewrite ltnn.
+Qed.
+
+
+
+Section Tamari.
+
+Variable n : nat.
+Implicit Type t : bintreesz n.
+
+Definition Tamari := connect (fun t1 t2 : bintreesz n => grel rotations t1 t2).
+Local Notation "x '<=T' y" := (Tamari x y) (at level 70, y at next level).
+
+Lemma Tamari_rotations t t' :
+  val t' \in rotations t -> t <=T t'.
+Proof. by move=> H; apply connect1; rewrite /grel /=. Qed.
+
+Lemma Tamari_refl : reflexive Tamari.
+Proof. exact: connect0. Qed.
+
+Lemma Tamari_trans : transitive Tamari.
+Proof. exact: connect_trans. Qed.
+
+Lemma Tamari_sumsizeleft t1 t2 :
+  t1 <=T t2 -> sumsizeleft t2 <= sumsizeleft t1 ?= iff (t1 == t2).
+Proof.
+move/connectP => [] /= p.
+elim: p t1 t2 => [| t0 p IHp] t1 t2 /=.
+  by move=> _ /= ->; split; rewrite // !eq_refl.
+move=> /andP [/sumsizeleft_gt Hgt /IHp H/H{IHp H}].
+move=> [] /leq_ltn_trans/(_ Hgt) Hlt _ {Hgt}.
+split; first exact: (ltnW Hlt).
+have:= Hlt; rewrite ltn_neqAle => /andP [/negbTE -> _].
+by case: eqP Hlt => [->|] //; rewrite ltnn.
+Qed.
+
+Lemma Tamari_anti : antisymmetric Tamari.
+Proof.
+move=> t1 t2 /andP [ /Tamari_sumsizeleft [leq21 eq]].
+move=> /Tamari_sumsizeleft [leq12 _].
+by apply/eqP; rewrite -eq eqn_leq leq21 leq12.
+Qed.
+
+Local Fact size_rightcombE : size_tree (rightcomb n) == n.
+Proof. apply/eqP; exact: size_rightcomb. Qed.
+Canonical rightcombsz := BinTreeSZ size_rightcombE.
+Local Fact size_leftcombE : size_tree (leftcomb n) == n.
+Proof. apply/eqP; exact: size_leftcomb. Qed.
+Canonical leftcombsz := BinTreeSZ size_leftcombE.
+Local Lemma size_flipE t : size_tree (flip t) == n.
+Proof. by rewrite size_flip bintreeszP. Qed.
+Canonical flipsz t := BinTreeSZ (size_flipE t).
+
+Lemma flipszK : involutive flipsz.
+Proof. move=> t; apply val_inj => /=; exact: flipK. Qed.
+
+Lemma Tamari_flip_impl t1 t2 : (flipsz t2 <=T flipsz t1) -> t1 <=T t2.
+Proof.
+rewrite /Tamari => /connectP /= [].
+case/lastP => [//= _ | p l Hp].
+  move=> /(congr1 flipsz); rewrite !flipszK => ->.
+  exact: connect0.
+rewrite last_rcons => Hl; subst l; move: Hp.
+have /eq_path -> :
+    (fun t t' => val t' \in rotations t)
+    =2 (fun t t' => (fun t' t => val (flipsz t) \in rotations (flipsz t')) t' t).
+  by move=> t t' /=; exact: rotation_flip.
+rewrite -rev_path /= last_rcons belast_rcons.
+have -> : (rev (flipsz t2 :: p)) =
+          [seq flipsz t | t <- rcons [seq flipsz t' | t' <- rev p] t2].
+  rewrite -[RHS]revK; congr rev.
+  rewrite -map_rev rev_rcons /= -map_rev revK.
+  rewrite -map_comp (eq_map (f2 := id)); last by move=> x /=; rewrite flipszK.
+  by rewrite map_id.
+rewrite (map_path (b := pred0)
+                  (e' := (fun t t' => val t' \in rotations t))); first last.
+  - by apply/hasP => [] [t /=].
+  - by rewrite /rel_base => u v _; rewrite /= !flipK.
+set pp := rcons _ _ => Hp; apply/connectP; exists pp; first by [].
+by rewrite /pp last_rcons.
+Qed.
+
+Lemma Tamari_flip t1 t2 : (flipsz t2 <=T flipsz t1) = (t1 <=T t2).
+Proof.
+apply/idP/idP; first exact: Tamari_flip_impl.
+rewrite -{1}(flipszK t1) -{1}(flipszK t2).
+exact: Tamari_flip_impl.
+Qed.
+
+Lemma rightcomb_bottom t : t <=T rightcombsz.
+Proof.
+move: {2}#|_| (leqnn #|[set t' | t <=T t' & t != t']|) => bound.
+elim: bound t => [| b IHb] t.
+  rewrite leqn0 cards_eq0 => /eqP Hlt.
+  have {Hlt} : rotations t == [::].
+    case Hrot : (rotations t) => [//| t0 r]; exfalso.
+    have {Hrot} Hrot : t0 \in rotations t by rewrite Hrot; exact: mem_head.
+    move/eqP : (size_rotations Hrot); rewrite bintreeszP => Ht0.
+    pose t' := BinTreeSZ Ht0.
+    have : t' \in [set t' | t <=T t' & t != t'].
+      rewrite inE; rewrite Tamari_rotations //=.
+      apply (introN idP) => /eqP /(congr1 val) /= Ht.
+      by move/rotations_neq: Hrot; rewrite Ht eq_refl.
+    by rewrite Hlt inE.
+  rewrite rightcomb_rotations => /eqP Ht.
+  suff -> : t = rightcombsz by exact: Tamari_refl.
+  by apply val_inj; rewrite /= Ht bintreeszP.
+move=> Hleq.
+case: (leqP #|[set t' | t <=T t' & t != t']| b) => [| Hlt]; first exact: IHb.
+have {Hleq Hlt} Hcard : #|[set t' | t <=T t' & t != t']| = b.+1.
+  by apply anti_leq; rewrite Hleq Hlt.
+case Hrot : (rotations t) => [| t0 s].
+  exfalso => {IHb}.
+  have {Hcard} : #|[set t' | t <=T t' & t != t']| > 0 by rewrite Hcard.
+  rewrite card_gt0 => /set0Pn [/= t0].
+  rewrite inE => /andP [].
+  rewrite /Tamari => /connectP [] [_ /= ->|t1 s] /=; first by rewrite eq_refl.
+  by rewrite Hrot in_nil.
+have {Hrot} Hrot : t0 \in rotations t by rewrite Hrot; exact: mem_head.
+move/eqP : (size_rotations Hrot); rewrite bintreeszP => Ht0.
+pose t' := BinTreeSZ Ht0.
+have:= Hrot; rewrite -[t0]/(val t') => /Tamari_rotations/Tamari_trans.
+apply; apply: IHb.
+rewrite -ltnS -{}Hcard; apply proper_card.
+rewrite /proper; apply/andP; split; apply/subsetP.
+- move=> /= z; rewrite !inE => /andP [Ht'z Hneq].
+  have Htz : t <=T z by apply: (Tamari_trans _ Ht'z); exact: Tamari_rotations.
+  rewrite Htz /=.
+  move: Hneq; apply contra => /eqP Heq; subst z.
+  apply/eqP; apply Tamari_anti; rewrite Ht'z /=.
+  exact: Tamari_rotations.
+- move/(_ t'); rewrite !inE.
+  rewrite eq_refl /= andbF => H; apply not_false_is_true; apply: H.
+  apply/andP; split; first exact: Tamari_rotations.
+  exact: rotations_neq.
+Qed.
+
+Lemma leftcomb_top t : leftcombsz <=T t.
+Proof.
+rewrite -Tamari_flip.
+suff -> : flipsz leftcombsz = rightcombsz by exact: rightcomb_bottom.
+by apply val_inj => /=; exact: flip_leftcomb.
+Qed.
+
